cleanup ZFC module, more boolean algebra proofs

DAO/Rocq/src/Classical/Theory/ZFC.v
@@ -1,1067 +1,1112 @@
 Require Import DAO.Core.ClassicalAlphaType.
 Require Import DAO.Core.ClassicalAlphaProperties.
+From Stdlib Require Import Lia.
+From Stdlib Require Import PeanoNat.
+From Stdlib Require Import Arith.
+From Stdlib Require Import List.
+Import ListNotations.
 
-(* ZFC in ClassicalAlphaType *)
-(* Embedding ZFC in ClassicalAlphaType by using the classical veil *)
 
-Section ZFC_in_ClassicalAlpha.
-Context `{H_alpha: ClassicalAlphaType}.
+(** * ZFC in ClassicalAlphaType
+    
+    This module shows that ZFC set theory naturally lives inside ClassicalAlphaType,
+    with the empty set being exactly classical_veil - the one impossible predicate. *)
 
-(* Sets are just predicates - rename to avoid conflict with Coq's Set *)
-Definition ZSet := AlphaPred.
+Module ZFC.
 
-(* Membership is predicate application *)
-Definition In (x : Alphacarrier) (A : ZSet) : Prop := A x.
-Notation "x 'in' A" := (In x A) (at level 70).
-Notation "x 'notin' A" := (~ In x A) (at level 70).
-
-(* Set equality via extensionality *)
-Definition set_eq (A B : ZSet) : Prop := pred_equiv A B.
-Notation "A == B" := (set_eq A B) (at level 70).
-
-(* Axiom 1: Extensionality (but it's just pred_equiv!) *)
-Theorem extensionality : forall A B : ZSet,
-  (forall x, x in A <-> x in B) <-> A == B.
-Proof.
-  intros A B.
-  unfold set_eq, pred_equiv, In.
-  split; intro H; exact H.
-Qed.
-
-(* Axiom 2: Empty Set (it's classical_veil!) *)
-Definition Empty : ZSet := classical_veil.
-
-Theorem empty_set_exists : exists E : ZSet, forall x, x notin E.
-Proof.
-  exists Empty.
-  intros x.
-  unfold In, Empty.
-  apply classical_veil_is_impossible.
-Qed.
-
-(* Singleton sets *)
-Definition singleton (a : Alphacarrier) : ZSet :=
-  fun x => x = a.
-
-Theorem singleton_spec : forall a x,
-  x in singleton a <-> x = a.
-Proof.
-  intros a x.
-  unfold In, singleton.
-  split; intro H; exact H.
-Qed.
-
-(* Now let's try pairing *)
-Definition pair (a b : Alphacarrier) : ZSet :=
-  fun x => x = a \/ x = b.
-
-Theorem pair_spec : forall a b x,
-  x in pair a b <-> (x = a \/ x = b).
-Proof.
-  intros a b x.
-  unfold In, pair.
-  split; intro H; exact H.
-Qed.
-
-
-(* Prove singletons are not empty (when element exists) *)
-Theorem singleton_not_empty : forall a,
- ~ (singleton a == Empty).
-Proof.
- intros a H_eq.
- (* If singleton a == Empty, then a in singleton a <-> a in Empty *)
- assert (a in singleton a) by (apply singleton_spec; reflexivity).
- assert (a in Empty) by (apply H_eq; exact H).
- (* But nothing is in Empty *)
- unfold In, Empty in H0.
- apply (classical_veil_is_impossible a).
- exact H0.
-Qed.
-
-(* Prove pairs are not empty *)
-Theorem pair_not_empty : forall a b,
- ~ (pair a b == Empty).
-Proof.
- intros a b H_eq.
- assert (a in pair a b) by (apply pair_spec; left; reflexivity).
- assert (a in Empty) by (apply H_eq; exact H).
- unfold In, Empty in H0.
- apply (classical_veil_is_impossible a).
- exact H0.
-Qed.
-
-(* Axiom 3: Pairing - we can form pairs! *)
-Theorem pairing_axiom : forall a b,
- exists P : ZSet, forall x, x in P <-> (x = a \/ x = b).
-Proof.
- intros a b.
- exists (pair a b).
- intro x.
- apply pair_spec.
-Qed.
-
-(* Define subset relation *)
-Definition subset (A B : ZSet) : Prop :=
- forall x, x in A -> x in B.
-Notation "A 'subseteq' B" := (subset A B) (at level 70).
-
-(* Binary union *)
-Definition union2 (A B : ZSet) : ZSet :=
- fun x => x in A \/ x in B.
-
-Theorem union2_spec : forall A B x,
- x in union2 A B <-> (x in A \/ x in B).
-Proof.
- intros A B x.
- unfold In, union2.
- split; intro H; exact H.
-Qed.
-
-(* Intersection *)
-Definition inter2 (A B : ZSet) : ZSet :=
- fun x => x in A /\ x in B.
-
-Theorem inter2_spec : forall A B x,
- x in inter2 A B <-> (x in A /\ x in B).
-Proof.
- intros A B x.
- unfold In, inter2.
- split; intro H; exact H.
-Qed.
-
-(* Set difference *)
-Definition diff (A B : ZSet) : ZSet :=
- fun x => x in A /\ x notin B.
-
-Theorem diff_spec : forall A B x,
- x in diff A B <-> (x in A /\ x notin B).
-Proof.
- intros A B x.
- unfold In, diff.
- split; intro H; exact H.
-Qed.
-
-(* Complement (relative to universal set) *)
-Definition compl (A : ZSet) : ZSet :=
- fun x => x notin A.
-
-(* The universal set is the_necessary! *)
-Definition Universal : ZSet := the_necessary.
-
-Theorem universal_contains_all : forall x,
- x in Universal.
-Proof.
- intros x.
- unfold In, Universal, the_necessary.
- apply classical_veil_is_impossible.
-Qed.
-
-(* Basic set algebra theorems *)
-Theorem union_empty_left : forall A,
- union2 Empty A == A.
-Proof.
- intros A.
- unfold set_eq, pred_equiv.
- intros x.
- split.
- - intros [H_empty | H_A].
-   + (* x in Empty - impossible *)
-     unfold In, Empty in H_empty.
-     exfalso.
-     apply (classical_veil_is_impossible x).
-     exact H_empty.
-   + exact H_A.
- - intros H_A.
-   right. exact H_A.
-Qed.
-
-Theorem inter_empty_left : forall A,
- inter2 Empty A == Empty.
-Proof.
- intros A.
- unfold set_eq, pred_equiv.
- intros x.
- split.
- - intros [H_empty H_A].
-   exact H_empty.
- - intros H_empty.
-   split.
-   + exact H_empty.
-   + (* Need to show x in A, but we know x in Empty which is impossible *)
-     unfold In, Empty in H_empty.
-     exfalso.
-     apply (classical_veil_is_impossible x).
-     exact H_empty.
-Qed.
-
-(* De Morgan's laws for sets *)
-Theorem de_morgan_union : forall A B,
-  compl (union2 A B) == inter2 (compl A) (compl B).
-Proof.
-  intros A B.
-  unfold set_eq, pred_equiv.
-  intros x.
-  unfold In, compl, union2, inter2.
-  (* Now we have: ~ (A x \/ B x) <-> ~ A x /\ ~ B x *)
-  split.
-  - (* Forward direction *)
-    intros H_not_union.
-    split.
-    + intros H_A. 
-      apply H_not_union.
-      left. exact H_A.
-    + intros H_B.
-      apply H_not_union.
-      right. exact H_B.
-  - (* Backward direction *)
-    intros [H_not_A H_not_B] [H_A | H_B].
-    + exact (H_not_A H_A).
-    + exact (H_not_B H_B).
-Qed.
-
-Theorem de_morgan_inter : forall A B,
-  compl (inter2 A B) == union2 (compl A) (compl B).
-Proof.
-  intros A B.
-  unfold set_eq, pred_equiv.
-  intros x.
-  unfold In, compl, inter2, union2.
-  (* Now we have: ~ (A x /\ B x) <-> ~ A x \/ ~ B x *)
-  split.
-  - (* Forward direction - need classical logic here *)
-    intros H_not_inter.
-    destruct (alpha_constant_decision (A x)) as [H_A | H_not_A].
-    + (* If A x, then must have ~ B x *)
-      right.
-      intros H_B.
-      apply H_not_inter.
-      split; assumption.
-    + (* If ~ A x, we're done *)
-      left. exact H_not_A.
-  - (* Backward direction *)
-    intros [H_not_A | H_not_B] [H_A H_B].
-    + exact (H_not_A H_A).
-    + exact (H_not_B H_B).
-Qed.
-
-
-(* Axiomatize that some elements of Alphacarrier can represent sets *)
-(* This is like saying "some elements are sets" in ZFC *)
-Axiom is_set_code : Alphacarrier -> Prop.
-Axiom set_decode : Alphacarrier -> ZSet.
-
-(* set_decode is only meaningful for set codes *)
-Axiom decode_only_codes : forall x,
-  ~ is_set_code x -> set_decode x == Empty.
-
-(* For any predicate that's "set-like", there's a code for it *)
-Axiom set_encode_exists : forall (S : ZSet), 
-  (exists a, S a) \/ (forall a, ~ S a) ->  (* S is not "middle" *)
-  exists x, is_set_code x /\ set_decode x == S.
-
-(* The membership relation for coded sets *)
-Definition mem (a b : Alphacarrier) : Prop :=
-  is_set_code b /\ a in set_decode b.
-
-Notation "a 'mem' b" := (mem a b) (at level 70).
-
-(* Let's verify this works with basic examples *)
-Theorem empty_set_has_code : 
-  exists e, is_set_code e /\ set_decode e == Empty.
-Proof.
-  apply set_encode_exists.
-  right. intros a H.
-  unfold Empty, In, classical_veil in H.
-  apply (classical_veil_is_impossible a H).
-Qed.
-
-(* Basic theorems about set codes *)
-Theorem singleton_has_code : forall a,
-  exists s, is_set_code s /\ set_decode s == singleton a.
-Proof.
-  intro a.
-  apply set_encode_exists.
-  left. exists a. 
-  unfold singleton, In. reflexivity.
-Qed.
-
-Theorem pair_has_code : forall a b,
-  exists p, is_set_code p /\ set_decode p == pair a b.
-Proof.
-  intros a b.
-  apply set_encode_exists.
-  left. exists a.
-  unfold pair, In. left. reflexivity.
-Qed.
-
-(* Union axiom - for any set of sets, their union exists *)
-Definition is_union_of (F union_set : Alphacarrier) : Prop :=
-  is_set_code F /\ is_set_code union_set /\
-  forall x, x mem union_set <-> exists Y, Y mem F /\ x mem Y.
-
-Axiom union_exists : forall F,
-  is_set_code F ->
-  exists U, is_union_of F U.
-
-
-(* Binary union as a special case *)
-Theorem binary_union_exists : forall A B,
-  is_set_code A -> is_set_code B ->
-  exists U, is_set_code U /\ 
-    forall x, x mem U <-> (x mem A \/ x mem B).
-Proof.
-  intros A B HA HB.
-  (* First, create a pair {A, B} *)
-  destruct (pair_has_code A B) as [P [HP HPdecode]].
-  (* Then take union of this pair *)
-  destruct (union_exists P HP) as [U HU].
-  exists U.
-  destruct HU as [HF [HUcode HUspec]].
-  split; [exact HUcode|].
-  intro x.
-  split.
-  - intro HxU.
-    apply HUspec in HxU.
-    destruct HxU as [Y [HYP HxY]].
-    (* Y mem P means is_set_code P /\ Y in set_decode P *)
-    destruct HYP as [_ HYP'].
-    (* Use HPdecode as a function *)
-    assert (Y in pair A B).
-    { apply HPdecode. exact HYP'. }
-    apply pair_spec in H.
-    destruct H as [HYA | HYB].
-    + left. subst Y. exact HxY.
-    + right. subst Y. exact HxY.
-  - intros [HxA | HxB].
-    + apply HUspec.
-      exists A. split; [|exact HxA].
-      split; [exact HP|].
-      (* Again, use HPdecode as a function *)
-      apply HPdecode.
-      apply pair_spec. left. reflexivity.
-    + apply HUspec.
-      exists B. split; [|exact HxB].
-      split; [exact HP|].
-      apply HPdecode.
-      apply pair_spec. right. reflexivity.
-Qed.
-
-(* Separation axiom schema - for any set and property, we can form the subset *)
-Axiom separation : forall A (P : Alphacarrier -> Prop),
-  is_set_code A ->
-  exists B, is_set_code B /\
-    forall x, x mem B <-> (x mem A /\ P x).
-
-(* Example: intersection via separation *)
-Theorem intersection_exists : forall A B,
-  is_set_code A -> is_set_code B ->
-  exists I, is_set_code I /\
-    forall x, x mem I <-> (x mem A /\ x mem B).
-Proof.
-  intros A B HA HB.
-  apply (separation A (fun x => x mem B) HA).
-Qed.
-
-
-(* First, let's define the successor operation in set theory *)
-(* Successor of x is x union {x} *)
-Definition is_successor (x sx : Alphacarrier) : Prop :=
-  is_set_code x /\ is_set_code sx /\
-  forall y, y mem sx <-> (y mem x \/ y = x).
-
-(* The axiom of infinity: there exists an inductive set *)
-(* A set is inductive if it contains empty and is closed under successor *)
-Definition is_inductive (I : Alphacarrier) : Prop :=
-  is_set_code I /\
-  (exists e, is_set_code e /\ (forall x, ~ (x mem e)) /\ e mem I) /\  (* contains empty *)
-  (forall x, x mem I -> exists sx, is_successor x sx /\ sx mem I).      (* closed under successor *)
-
-Axiom infinity : exists I, is_inductive I.
-
-(* Direct axiomatization of important set codes *)
-Axiom empty_code : Alphacarrier.
-Axiom empty_code_spec : is_set_code empty_code /\ set_decode empty_code == Empty.
-
-(* Similarly for other constructions *)
-Axiom singleton_code : Alphacarrier -> Alphacarrier.
-Axiom singleton_code_spec : forall a,
-  is_set_code (singleton_code a) /\ 
-  set_decode (singleton_code a) == singleton a.
-
-Axiom pair_code : Alphacarrier -> Alphacarrier -> Alphacarrier.
-Axiom pair_code_spec : forall a b,
-  is_set_code (pair_code a b) /\ 
-  set_decode (pair_code a b) == pair a b.
-
-Axiom successor_code : Alphacarrier -> Alphacarrier.
-Axiom successor_code_spec : forall x,
-  is_set_code x -> is_successor x (successor_code x).
-
-(* Alternative approach - let's make a cleaner lemma first *)
-Lemma not_mem_empty : forall x, ~ (x mem empty_code).
-Proof.
-  intros x [Hcode Hin].
-  destruct empty_code_spec as [_ Hdecode].
-  apply Hdecode in Hin.
-  unfold In, Empty in Hin.
-  exact (classical_veil_is_impossible x Hin).
-Qed.
-
-(* Now the theorem is trivial *)
-Theorem zero_exists_zfc : exists z,
-  is_set_code z /\ forall x, ~ (x mem z).
-Proof.
-  exists empty_code.
-  destruct empty_code_spec as [Hcode _].
-  split.
-  - exact Hcode.
-  - exact not_mem_empty.
-Qed.
-
-(* Let's build the first few natural numbers explicitly *)
-Definition zero_zfc := empty_code.
-Definition one_zfc := successor_code zero_zfc.
-Definition two_zfc := successor_code one_zfc.
-Definition three_zfc := successor_code two_zfc.
-
-(* Prove basic properties *)
-Lemma zero_is_empty : forall x, ~ (x mem zero_zfc).
-Proof.
-  exact not_mem_empty.
-Qed.
-
-Lemma one_contains_only_zero : forall x,
-  x mem one_zfc <-> x = zero_zfc.
-Proof.
-  intro x.
-  unfold one_zfc.
-  destruct empty_code_spec as [Hcode _].
-  destruct (successor_code_spec zero_zfc Hcode) as [_ [Hscode Hspec]].
-  split.
-  - intro Hmem.
-    apply Hspec in Hmem.
-    destruct Hmem as [Hcontra | Heq].
-    + exfalso. exact (zero_is_empty x Hcontra).
-    + exact Heq.
-  - intro Heq.
-    subst x.
-    apply Hspec.
-    right. reflexivity.
-Qed.
-
-Lemma two_contains_zero_and_one : forall x,
-  x mem two_zfc <-> (x = zero_zfc \/ x = one_zfc).
-Proof.
-  intro x.
-  unfold two_zfc, one_zfc.
-  (* Get the properties of successor_code *)
-  destruct empty_code_spec as [Hcode0 _].
-  
-  (* First application of successor_code_spec *)
-  assert (Hsucc1 := successor_code_spec zero_zfc Hcode0).
-  destruct Hsucc1 as [_ [Hcode_one Hspec1]].
-  (* Now Hcode_one : is_set_code (successor_code zero_zfc) *)
-  
-  (* Second application of successor_code_spec *)
-  assert (Hsucc2 := successor_code_spec (successor_code zero_zfc) Hcode_one).
-  destruct Hsucc2 as [_ [Hcode_two Hspec2]].
-  
-  split.
-  - intro Hmem.
-    apply Hspec2 in Hmem.
-    destruct Hmem as [Hin1 | Heq1].
-    + (* x mem one_zfc *)
-      apply one_contains_only_zero in Hin1.
-      left. exact Hin1.
-    + (* x = one_zfc *)
-      right. exact Heq1.
-  - intros [Hz | Ho].
-    + (* x = zero_zfc *)
-      subst x.
-      apply Hspec2.
-      left.
-      apply one_contains_only_zero.
-      reflexivity.
-    + (* x = one_zfc *)
-      subst x.
-      apply Hspec2.
-      right. reflexivity.
-Qed.
-
-(* Axiom: empty sets have unique codes *)
-Axiom empty_unique : forall e1 e2,
-  is_set_code e1 -> is_set_code e2 ->
-  (forall x, ~ (x mem e1)) ->
-  (forall x, ~ (x mem e2)) ->
-  e1 = e2.
-
-(* The natural numbers are the intersection of all inductive sets *)
-Definition is_natural_number (n : Alphacarrier) : Prop :=
-  forall I, is_inductive I -> n mem I.
-
-Theorem zero_is_natural : is_natural_number zero_zfc.
-Proof.
-  unfold is_natural_number, zero_zfc.
-  intros I HI.
-  destruct HI as [HIcode [[e [He [Hemp Hemem]]] Hclosed]].
-  (* Both empty_code and e are empty sets *)
-  assert (e = empty_code).
-  { apply empty_unique.
-    - exact He.
-    - destruct empty_code_spec; assumption.
-    - exact Hemp.
-    - exact not_mem_empty. }
-  subst e.
-  exact Hemem.
-Qed.
-
-(* Supporting axioms we need for natural numbers *)
-Axiom nat_set_code : Alphacarrier.
-Axiom nat_set_code_spec : 
-  is_set_code nat_set_code /\
-  forall n, n mem nat_set_code <-> is_natural_number n.
-
-Axiom nat_is_set_code : forall n,
-  is_natural_number n -> is_set_code n.
-
-Axiom successor_preserves_nat : forall n,
-  is_natural_number n -> is_natural_number (successor_code n).
-
-(* Induction principle for natural numbers *)
-Theorem nat_induction_zfc : forall (P : Alphacarrier -> Prop),
-  P zero_zfc ->
-  (forall n, is_natural_number n -> P n -> P (successor_code n)) ->
-  forall n, is_natural_number n -> P n.
-Proof.
-  intros P Hz Hsucc n Hn.
-  
-  (* The subset of naturals satisfying P *)
-  destruct nat_set_code_spec as [Hnat_code Hnat_spec].
-  destruct (separation nat_set_code P Hnat_code) as [S [HS HSspec]].
-  
-  (* Claim: S is inductive *)
-  assert (His_ind: is_inductive S).
-  { unfold is_inductive.
-    split; [exact HS|].
-    split.
-    - (* S contains empty/zero *)
-      exists zero_zfc.
-      split; [|split].
-      + destruct empty_code_spec; assumption.
-      + exact zero_is_empty.
-      + apply HSspec. split.
-        * apply Hnat_spec. exact zero_is_natural.
-        * exact Hz.
-    - (* S is closed under successor *)
-      intros x HxS.
-      (* Extract the components without modifying HxS *)
-      assert (Hx_components: x mem nat_set_code /\ P x).
-      { apply HSspec. exact HxS. }
-      destruct Hx_components as [Hx_in_nat Px].
+  (** ** Basic Definitions
       
-      assert (Hx_nat: is_natural_number x).
-      { apply Hnat_spec. exact Hx_in_nat. }
+      Sets are predicates, membership is predicate application *)
+  Module Basic.
+    Section BasicDefs.
+      Context {H_alpha: ClassicalAlphaType}.
       
-      assert (Hx_code: is_set_code x).
-      { apply nat_is_set_code. exact Hx_nat. }
+      (* Sets are just predicates *)
+      Definition ZSet := ClassicalAlphaProperties.Helpers.AlphaPred.
       
-      exists (successor_code x).
-      split.
-      + apply successor_code_spec. exact Hx_code.
-      + apply HSspec. split.
-        * apply Hnat_spec. 
-          apply successor_preserves_nat. exact Hx_nat.
-        * apply Hsucc.
-          -- exact Hx_nat.
-          -- exact Px. }
-  
-  (* Since n is natural, it's in S *)
-  assert (n_in_S: n mem S).
-  { unfold is_natural_number in Hn.
-    exact (Hn S His_ind). }
-  
-  (* Therefore P n holds *)
-  apply HSspec in n_in_S.
-  destruct n_in_S as [_ Pn].
-  exact Pn.
-Qed.
+      (* Membership is predicate application *)
+      Definition In (x : Alphacarrier) (A : ZSet) : Prop := A x.
+      
+      (* Set equality via extensionality *)
+      Definition set_eq (A B : ZSet) : Prop := 
+        ClassicalAlphaProperties.Predicates.pred_equiv A B.
+      
+      (* Axiom 1: Extensionality (but it's just pred_equiv!) *)
+      Theorem extensionality : forall A B : ZSet,
+        (forall x, In x A <-> In x B) <-> set_eq A B.
+      Proof.
+        intros A B.
+        unfold set_eq, ClassicalAlphaProperties.Predicates.pred_equiv, In.
+        split; intro H; exact H.
+      Qed.
+      
+    End BasicDefs.
+  End Basic.
 
-(* First, let's properly handle subset encoding *)
-Definition encodes_subset (x : Alphacarrier) (A : Alphacarrier) : Prop :=
-  is_set_code x /\ is_set_code A /\
-  forall y, y mem x -> y mem A.
+  (** ** Fundamental Sets
+      
+      The empty set (classical_veil) and basic constructions *)
+  Module Fundamental.
+    Section FundamentalSets.
+      Context {H_alpha: ClassicalAlphaType}.
+      Import Basic.
+      
+      (* The empty set is classical_veil! *)
+      Definition Empty : ZSet := classical_veil.
+      
+      Theorem empty_set_exists : exists E : ZSet, forall x, ~ In x E.
+      Proof.
+        exists Empty.
+        intros x.
+        unfold In, Empty.
+        apply ClassicalAlphaProperties.Core.classical_veil_is_impossible.
+      Qed.
+      
+      (* Singleton sets *)
+      Definition singleton (a : Alphacarrier) : ZSet :=
+        fun x => x = a.
+      
+      Theorem singleton_spec : forall a x,
+        In x (singleton a) <-> x = a.
+      Proof.
+        intros a x.
+        unfold In, singleton.
+        split; intro H; exact H.
+      Qed.
+      
+      (* Pairing *)
+      Definition pair (a b : Alphacarrier) : ZSet :=
+        fun x => x = a \/ x = b.
+      
+      Theorem pair_spec : forall a b x,
+        In x (pair a b) <-> (x = a \/ x = b).
+      Proof.
+        intros a b x.
+        unfold In, pair.
+        split; intro H; exact H.
+      Qed.
+      
+      (* Basic non-emptiness results *)
+      Theorem singleton_not_empty : forall a,
+        ~ (set_eq (singleton a) Empty).
+      Proof.
+        intros a H_eq.
+        assert (In a (singleton a)) by (apply singleton_spec; reflexivity).
+        assert (In a Empty) by (apply H_eq; exact H).
+        unfold In, Empty in H0.
+        apply (ClassicalAlphaProperties.Core.classical_veil_is_impossible a).
+        exact H0.
+      Qed.
 
-(* Power set: collection of all subsets of A *)
-Definition is_powerset (A ps : Alphacarrier) : Prop :=
-  is_set_code A /\ is_set_code ps /\
-  forall x, x mem ps <-> encodes_subset x A.
+    End FundamentalSets.
+  End Fundamental.
 
-(* Power Set Axiom *)
-Axiom powerset_exists : forall A,
-  is_set_code A -> exists ps, is_powerset A ps.
+  (** ** Set Operations
+      
+      Union, intersection, complement, etc. *)
+  Module Operations.
+    Section SetOperations.
+      Context {H_alpha: ClassicalAlphaType}.
+      Import Basic.
+      Import Fundamental.
+      
+      (* Define subset relation *)
+      Definition subset (A B : ZSet) : Prop :=
+        forall x, In x A -> In x B.
+      
+      (* Binary union *)
+      Definition union2 (A B : ZSet) : ZSet :=
+        fun x => In x A \/ In x B.
+      
+      Theorem union2_spec : forall A B x,
+        In x (union2 A B) <-> (In x A \/ In x B).
+      Proof.
+        intros A B x.
+        unfold In, union2.
+        split; intro H; exact H.
+      Qed.
+      
+      (* Intersection *)
+      Definition inter2 (A B : ZSet) : ZSet :=
+        fun x => In x A /\ In x B.
+      
+      Theorem inter2_spec : forall A B x,
+        In x (inter2 A B) <-> (In x A /\ In x B).
+      Proof.
+        intros A B x.
+        unfold In, inter2.
+        split; intro H; exact H.
+      Qed.
+      
+      (* Complement *)
+      Definition compl (A : ZSet) : ZSet :=
+        fun x => ~ In x A.
+      
+      (* The universal set *)
+      Definition Universal : ZSet := 
+        ClassicalAlphaProperties.Helpers.the_necessary.
+      
+      Theorem universal_contains_all : forall x,
+        In x Universal.
+      Proof.
+        intros x.
+        unfold In, Universal, ClassicalAlphaProperties.Helpers.the_necessary.
+        apply ClassicalAlphaProperties.Core.classical_veil_is_impossible.
+      Qed.
+    End SetOperations.
+  End Operations.
 
-(* Let's prove some basic properties *)
-Theorem empty_in_every_powerset : forall A ps,
-  is_set_code A -> is_powerset A ps ->
-  empty_code mem ps.
-Proof.
-  intros A ps HA Hps.
-  destruct Hps as [_ [Hps_code Hps_spec]].
-  apply Hps_spec.
-  unfold encodes_subset.
-  destruct empty_code_spec as [He_code _].
-  split; [exact He_code|].
-  split; [exact HA|].
-  intros y Hy.
-  (* y mem empty_code is impossible *)
-  exfalso.
-  exact (not_mem_empty y Hy).
-Qed.
-
-Theorem set_in_own_powerset : forall A ps,
-  is_set_code A -> is_powerset A ps ->
-  A mem ps.
-Proof.
-  intros A ps HA Hps.
-  destruct Hps as [_ [Hps_code Hps_spec]].
-  apply Hps_spec.
-  unfold encodes_subset.
-  split; [exact HA|].
-  split; [exact HA|].
-  intros y Hy.
-  (* y mem A -> y mem A is trivial *)
-  exact Hy.
-Qed.
-
-(* Singleton subsets *)
-(* Singleton subsets *)
-Theorem singleton_in_powerset : forall A ps a,
-  is_set_code A -> is_powerset A ps -> a mem A ->
-  exists sa, is_set_code sa /\ sa mem ps /\
-    forall x, x mem sa <-> x = a.
-Proof.
-  intros A ps a HA Hps Ha.
-  (* Get singleton code *)
-  exists (singleton_code a).
-  destruct (singleton_code_spec a) as [Hsa_code Hsa_decode].
-  split; [exact Hsa_code|].
-  split.
-  - (* singleton a is in powerset *)
-    destruct Hps as [_ [_ Hps_spec]].
-    apply Hps_spec.
-    unfold encodes_subset.
-    split; [exact Hsa_code|].
-    split; [exact HA|].
-    intros x Hx.
-    (* If x mem singleton a, then x = a, so x mem A *)
-    destruct Hx as [_ Hx_in].
-    assert (x in singleton a).
-    { apply Hsa_decode. exact Hx_in. }
-    (* Use singleton spec to get x = a *)
-    assert (x = a).
-    { apply singleton_spec. exact H. }
-    (* Now rewrite using the equality *)
-    rewrite H0.
-    exact Ha.
-  - (* Characterization of singleton *)
-    intros x.
-    split.
-    + intro Hx.
-      destruct Hx as [_ Hx_in].
-      assert (x in singleton a).
-      { apply Hsa_decode. exact Hx_in. }
-      apply singleton_spec.
-      exact H.
-    + intro Heq.
-      rewrite Heq.  (* Use rewrite instead of subst *)
-      split; [exact Hsa_code|].
-      apply Hsa_decode.
-      apply singleton_spec.
-      reflexivity.
-Qed.
-
-
-(* Replacement Axiom *)
-
-(* A relation is functional if it maps each input to at most one output *)
-Definition is_functional (R : Alphacarrier -> Alphacarrier -> Prop) : Prop :=
-  forall x y z, R x y -> R x z -> y = z.
-
-(* Replacement: The image of a set under a functional relation is a set *)
-Axiom replacement : forall A (R : Alphacarrier -> Alphacarrier -> Prop),
-  is_set_code A ->
-  is_functional R ->
-  exists B, is_set_code B /\
-    forall y, y mem B <-> exists x, x mem A /\ R x y.
-
-(* Example application: Construct {f(x) | x ∈ A} for any function f *)
-Definition function_image (A : Alphacarrier) (f : Alphacarrier -> Alphacarrier) : Prop :=
-  is_set_code A ->
-  exists B, is_set_code B /\
-    forall y, y mem B <-> exists x, x mem A /\ y = f x.
-
-Theorem function_image_exists : forall A f,
-  is_set_code A ->
-  exists B, is_set_code B /\
-    forall y, y mem B <-> exists x, x mem A /\ y = f x.
-Proof.
-  intros A f HA.
-  (* Define the relation R(x,y) := y = f(x) *)
-  pose (R := fun x y => y = f x).
-  (* Show R is functional *)
-  assert (Hfunc: is_functional R).
-  { unfold is_functional, R.
-    intros x y z Hy Hz.
-    (* Hy : y = f x, Hz : z = f x, so y = z by transitivity *)
-    rewrite Hy.
-    symmetry.
-    exact Hz. }
-  (* Apply replacement *)
-  destruct (replacement A R HA Hfunc) as [B [HB HBspec]].
-  exists B. split; [exact HB|].
-  intros y. split.
-  - intro HyB.
-    apply HBspec in HyB.
-    destruct HyB as [x [HxA Hy]].
-    exists x. split; [exact HxA|].
-    unfold R in Hy. exact Hy.
-  - intros [x [HxA Heq]].
-    apply HBspec.
-    exists x. split; [exact HxA|].
-    unfold R. exact Heq.
-Qed.
-
-(* Foundation/Regularity Axiom *)
-(* Every non-empty set has an ∈-minimal element *)
-Axiom foundation : forall A,
-  is_set_code A ->
-  (exists x, x mem A) ->
-  exists x, x mem A /\ forall y, y mem x -> ~ (y mem A).
-
-(* This prevents things like x ∈ x or infinite chains x₀ ∈ x₁ ∈ x₂ ∈ ... *)
-Theorem no_set_contains_itself : forall x,
-  is_set_code x -> ~ (x mem x).
-Proof.
-  intros x Hx Hmem.
-  (* Apply foundation to {x} *)
-  destruct (singleton_code_spec x) as [Hs_code Hs_decode].
-  assert (exists y, y mem singleton_code x).
-  { exists x. 
-    (* Need to show x mem singleton_code x *)
-    (* By definition, mem requires is_set_code and membership *)
-    split.
-    - exact Hs_code.
-    - apply Hs_decode.
-      apply singleton_spec.
-      reflexivity. }
-  destruct (foundation (singleton_code x) Hs_code H) as [y [Hy Hmin]].
-  (* y must be x since singleton only contains x *)
-  assert (y = x).
-  { destruct Hy as [_ Hy_in].
-    apply Hs_decode in Hy_in.
-    apply singleton_spec in Hy_in.
-    exact Hy_in. }
-  subst y.
-  (* But then x is minimal, so nothing in x is in singleton x *)
-  (* In particular, x in x implies x in singleton x, contradiction *)
-  apply (Hmin x Hmem).
-  (* Again, build mem without unfold *)
-  split.
-  - exact Hs_code.
-  - apply Hs_decode. 
-    apply singleton_spec. 
-    reflexivity.
-Qed.
-
-
-(* Axiom of Choice *)
-
-(* A family of sets is a set whose elements are all sets *)
-Definition is_family_of_sets (F : Alphacarrier) : Prop :=
-  is_set_code F /\ forall x, x mem F -> is_set_code x.
-
-(* A choice function selects one element from each set in the family *)
-Definition is_choice_function (F f : Alphacarrier) : Prop :=
-  is_family_of_sets F /\ is_set_code f /\
-  forall A, A mem F -> 
-    (exists a, a mem A) ->  (* if A is non-empty *)
-    exists a, a mem A /\ (pair_code A a) mem f.  (* f picks element a from A *)
-
-(* Axiom of Choice: Every family of non-empty sets has a choice function *)
-Axiom zf_choice : forall F,
-  is_family_of_sets F ->
-  (forall A, is_set_code A -> A in set_decode F -> exists a, is_set_code a /\ a in set_decode A) ->
-  exists f, is_choice_function F f.
-
-
-
-(* Define mem as a regular function since notation is problematic *)
-Definition is_member (a b : Alphacarrier) : Prop :=
-  is_set_code b /\ a in set_decode b.
-
-(* ============ Additional Theorems: Set Theory and Impossibility ============ *)
-
-(* Basic insight: any set containing empty is non-empty *)
-Theorem set_containing_void_not_void : forall A,
-  is_set_code A -> is_member empty_code A -> ~ (A = empty_code).
-Proof.
-  intros A HA Hmem Heq.
-  subst A.
-  (* is_member empty_code empty_code, but nothing is in empty *)
-  destruct Hmem as [_ Hin].
-  destruct empty_code_spec as [_ Hdecode].
-  apply Hdecode in Hin.
-  unfold In, Empty in Hin.
-  exact (classical_veil_is_impossible empty_code Hin).
-Qed.
-
-(* The complement of empty is universal *)
-Theorem complement_empty_is_universal :
-  compl Empty == Universal.
-Proof.
-  unfold set_eq, pred_equiv.
-  intro x.
-  unfold compl, Empty, Universal, In, the_necessary.
-  split.
-  - intro H. exact H.
-  - intro H. exact H.
-Qed.
-
-(* Russell's Paradox in our framework *)
-Definition russell_set : ZSet :=
-  fun x => is_set_code x /\ ~ (is_member x x).
-
-(* The Russell set cannot have a code! *)
-Theorem russell_has_no_code :
-  ~ exists r, is_set_code r /\ set_decode r == russell_set.
-Proof.
-  intros [r [Hr Hdecode]].
-  (* Consider: is_member r r *)
-  destruct (alpha_constant_decision (is_member r r)) as [Hmem | Hnmem].
-  - (* If is_member r r, then r in russell_set by Hdecode, so ~ (is_member r r) *)
-    assert (r in russell_set).
-    { apply Hdecode. destruct Hmem as [_ H]. exact H. }
-    unfold russell_set, In in H.
-    destruct H as [_ Hnot].
-    exact (Hnot Hmem).
-  - (* If ~ (is_member r r), then r satisfies russell_set *)
-    assert (r in russell_set).
-    { unfold russell_set, In. split; assumption. }
-    assert (is_member r r).
-    { split; [exact Hr|]. apply Hdecode. exact H. }
-    exact (Hnmem H0).
-Qed.
-
-(* This means Russell's set is "too big" - it would collapse to classical_veil *)
-Theorem russell_would_be_impossible :
-  forall r, is_set_code r -> 
-  (forall x, is_member x r <-> (is_set_code x /\ ~ (is_member x x))) ->
-  forall x, ~ (is_member x r).
-Proof.
-  intros r Hr Hspec x Hmem.
-  (* Same contradiction as above *)
-  destruct (alpha_constant_decision (is_member r r)) as [Hmemr | Hnmemr].
-  - (* If is_member r r *)
-    assert (Hrr_spec: is_set_code r /\ ~ is_member r r).
-    { apply Hspec. exact Hmemr. }
-    destruct Hrr_spec as [_ Hnot].
-    exact (Hnot Hmemr).
-  - (* If ~ is_member r r *)
-    assert (is_member r r).
-    { apply Hspec. split; assumption. }
-    exact (Hnmemr H).
-Qed.
-
-(* The von Neumann hierarchy: sets have "distance" from void *)
-Definition rank_0_set (x : Alphacarrier) : Prop :=
-  is_set_code x /\ forall y, ~ (is_member y x).
-
-Definition rank_at_most_n : nat -> Alphacarrier -> Prop :=
-  fix rank n x :=
-    match n with
-    | 0 => rank_0_set x
-    | S n' => is_set_code x /\ 
-              forall y, is_member y x -> rank n' y
-    end.
-
-(* Empty set has rank 0 *)
-Theorem empty_rank_0 : rank_at_most_n 0 empty_code.
-Proof.
-  unfold rank_at_most_n, rank_0_set.
-  destruct empty_code_spec as [Hcode _].
-  split.
-  - exact Hcode.
-  - intros y [Hy_code Hy_in].
-    destruct empty_code_spec as [_ Hdecode].
-    apply Hdecode in Hy_in.
-    unfold In, Empty in Hy_in.
-    exact (classical_veil_is_impossible y Hy_in).
-Qed.
-
-(* Singletons have rank 1 *)
-Theorem singleton_rank_1 : forall a,
-  rank_at_most_n 0 a ->
-  rank_at_most_n 1 (singleton_code a).
-Proof.
-  intros a H0.
-  simpl.
-  destruct (singleton_code_spec a) as [Hcode Hdecode].
-  split; [exact Hcode|].
-  intros y Hy.
-  (* is_member y (singleton_code a) means y = a *)
-  destruct Hy as [_ Hy_in].
-  assert (y in singleton a) by (apply Hdecode; exact Hy_in).
-  assert (y = a) by (apply singleton_spec; exact H).
-  subst y.
-  exact H0.
-Qed.
-
-(* The hierarchy is well-founded by Foundation axiom *)
-Theorem no_infinite_membership_descent : forall f : nat -> Alphacarrier,
-  (forall n, is_set_code (f n)) ->
-  ~ (forall n, is_member (f (S n)) (f n)).
-Proof.
-  intros f Hcodes Hdescent.
-  (* This would violate foundation - but the proof is complex *)
-  (* Key idea: the range of f would be a set with no minimal element *)
-Admitted. (* Would need more machinery *)
-
-
-(* Helper lemmas for converting between mem and is_member *)
-Lemma mem_to_is_member : forall a b,
-  a mem b -> is_member a b.
-Proof.
-  intros a b H.
-  exact H.
-Qed.
-
-Lemma is_member_to_in_decode : forall a b,
-  is_member a b -> is_set_code b /\ a in set_decode b.
-Proof.
-  intros a b H.
-  exact H.
-Qed.
-
-Lemma in_decode_to_mem : forall a b,
-  is_set_code b -> a in set_decode b -> a mem b.
-Proof.
-  intros a b Hcode Hin.
-  split; assumption.
-Qed.
-
-(* Helper for the diagonal argument *)
-Lemma diagonal_contradiction : forall A d D f,
-  is_set_code D ->
-  (forall x, x mem D <-> x mem A /\ ~ is_member x (f x)) ->
-  D = f d ->
-  is_member d D ->
-  False.
-Proof.
-  intros A d D f HD HDspec Heq [_ Hd_in].
-  (* Build d mem D *)
-  assert (d mem D) by (split; assumption).
-  (* Apply HDspec to get ~ is_member d (f d) *)
-  apply HDspec in H.
-  destruct H as [_ Hnot_fd].
-  (* But f d = D, so ~ is_member d D *)
-  rewrite <- Heq in Hnot_fd.
-  (* Contradiction: we have both is_member d D and ~ is_member d D *)
-  apply Hnot_fd.
-  split; assumption.
-Qed.
-
-(* Cantor's Theorem in our framework *)
-Theorem cantor_theorem : forall A ps,
-  is_set_code A -> is_powerset A ps ->
-  ~ exists f : Alphacarrier -> Alphacarrier,
-    (forall x, is_member x A -> is_member (f x) ps) /\
-    (forall y, is_member y ps -> exists x, is_member x A /\ y = f x).
-Proof.
-  intros A ps HA Hps [f [Hf_maps Hf_onto]].
-  
-  (* Define the diagonal set D = {x ∈ A | x ∉ f(x)} *)
-  destruct (separation A (fun x => ~ (is_member x (f x))) HA) as [D [HD HDspec]].
-  
-  (* D is a subset of A, so D ∈ P(A) *)
-  assert (HD_in_ps: is_member D ps).
-  { destruct Hps as [_ [_ Hps_spec]].
-    apply Hps_spec.
-    unfold encodes_subset.
-    split; [exact HD|].
-    split; [exact HA|].
-    intros y Hy.
-    (* Extract that y is in A *)
-    destruct Hy as [_ Hy_in].
-    assert (y mem D) by (split; assumption).
-    apply HDspec in H.
-    destruct H as [H_mem_A _].
-    exact H_mem_A. }
-  
-  (* Since f is onto, D = f(d) for some d ∈ A *)
-  destruct (Hf_onto D HD_in_ps) as [d [Hd Heq]].
-  
-  (* Now we get our contradiction: d ∈ D ↔ d ∉ f(d) = D *)
-  destruct (alpha_constant_decision (is_member d D)) as [Hd_in | Hd_out].
-  - (* d ∈ D, so d ∉ f(d) = D, contradiction *)
-    exact (diagonal_contradiction A d D f HD HDspec Heq Hd_in).
-  - (* d ∉ D, so d ∈ f(d) = D, contradiction *)
-    assert (is_member d D).
-    { split.
-      - exact HD.
-      - apply HDspec.
+  (** ** Set Algebra
+      
+      Basic theorems about set operations *)
+  Module Algebra.
+    Section SetAlgebra.
+      Context {H_alpha: ClassicalAlphaType}.
+      Import Basic.
+      Import Fundamental.
+      Import Operations.
+      
+      Theorem union_empty_left : forall A,
+        set_eq (union2 Empty A) A.
+      Proof.
+        intros A.
+        unfold set_eq, ClassicalAlphaProperties.Predicates.pred_equiv.
+        intros x.
         split.
-        + exact Hd.
-        + rewrite <- Heq. exact Hd_out. }
-    exact (Hd_out H).
-Qed.
+        - intros [H_empty | H_A].
+          + unfold In, Empty in H_empty.
+            exfalso.
+            apply (ClassicalAlphaProperties.Core.classical_veil_is_impossible x).
+            exact H_empty.
+          + exact H_A.
+        - intros H_A.
+          right. exact H_A.
+      Qed.
+      
+      (* De Morgan's laws *)
+      Theorem de_morgan_union : forall A B,
+        set_eq (compl (union2 A B)) (inter2 (compl A) (compl B)).
+      Proof.
+        intros A B.
+        unfold set_eq, ClassicalAlphaProperties.Predicates.pred_equiv.
+        intros x.
+        unfold In, compl, union2, inter2.
+        split.
+        - intros H_not_union.
+          split.
+          + intros H_A. 
+            apply H_not_union.
+            left. exact H_A.
+          + intros H_B.
+            apply H_not_union.
+            right. exact H_B.
+        - intros [H_not_A H_not_B] [H_A | H_B].
+          + exact (H_not_A H_A).
+          + exact (H_not_B H_B).
+      Qed.
+    End SetAlgebra.
+  End Algebra.
+
+  (** ** Set Codes
+      
+      Encoding sets as elements for higher-order constructions *)
+  Module Codes.
+    Section SetCodes.
+      Context {H_alpha: ClassicalAlphaType}.
+      Import Basic.
+      Import Fundamental.
+      
+      (* Axiomatize that some elements can represent sets *)
+      Axiom is_set_code : Alphacarrier -> Prop.
+      Axiom set_decode : Alphacarrier -> ZSet.
+      
+      (* set_decode is only meaningful for set codes *)
+      Axiom decode_only_codes : forall x,
+        ~ is_set_code x -> set_eq (set_decode x) Empty.
+      
+      (* For any predicate that's "set-like", there's a code for it *)
+      Axiom set_encode_exists : forall (S : ZSet), 
+        (exists a, In a S) \/ (forall a, ~ In a S) ->
+        exists x, is_set_code x /\ set_eq (set_decode x) S.
+      
+      (* The membership relation for coded sets *)
+      Definition mem (a b : Alphacarrier) : Prop :=
+        is_set_code b /\ In a (set_decode b).
+      
+      (* Direct axiomatization of important set codes *)
+      Axiom empty_code : Alphacarrier.
+      Axiom empty_code_spec : 
+        is_set_code empty_code /\ set_eq (set_decode empty_code) Empty.
+      
+      Axiom singleton_code : Alphacarrier -> Alphacarrier.
+      Axiom singleton_code_spec : forall a,
+        is_set_code (singleton_code a) /\ 
+        set_eq (set_decode (singleton_code a)) (singleton a).
+      
+      Axiom pair_code : Alphacarrier -> Alphacarrier -> Alphacarrier.
+      Axiom pair_code_spec : forall a b,
+        is_set_code (pair_code a b) /\ 
+        set_eq (set_decode (pair_code a b)) (pair a b).
+      
+      (* Helper lemmas *)
+      Lemma not_mem_empty : forall x, ~ mem x empty_code.
+      Proof.
+        intros x [Hcode Hin].
+        destruct empty_code_spec as [_ Hdecode].
+        apply Hdecode in Hin.
+        unfold In, Empty in Hin.
+        exact (ClassicalAlphaProperties.Core.classical_veil_is_impossible x Hin).
+      Qed.
+    End SetCodes.
+  End Codes.
+
+  (** ** Axioms
+      
+      The standard ZFC axioms in our framework *)
+  Module Axioms.
+    Section ZFCAxioms.
+      Context {H_alpha: ClassicalAlphaType}.
+      Import Basic.
+      Import Fundamental.
+      Import Operations.
+      Import Codes.
+      
+      (* Union axiom *)
+      Definition is_union_of (F union_set : Alphacarrier) : Prop :=
+        is_set_code F /\ is_set_code union_set /\
+        forall x, mem x union_set <-> exists Y, mem Y F /\ mem x Y.
+      
+      Axiom union_exists : forall F,
+        is_set_code F ->
+        exists U, is_union_of F U.
+      
+      (* Separation axiom schema *)
+      Axiom separation : forall A (P : Alphacarrier -> Prop),
+        is_set_code A ->
+        exists B, is_set_code B /\
+          forall x, mem x B <-> (mem x A /\ P x).
+      
+      (* Axiom of infinity *)
+      Definition is_successor (x sx : Alphacarrier) : Prop :=
+        is_set_code x /\ is_set_code sx /\
+        forall y, mem y sx <-> (mem y x \/ y = x).
+      
+      Definition is_inductive (I : Alphacarrier) : Prop :=
+        is_set_code I /\
+        (exists e, is_set_code e /\ (forall x, ~ mem x e) /\ mem e I) /\
+        (forall x, mem x I -> exists sx, is_successor x sx /\ mem sx I).
+      
+      Axiom infinity : exists I, is_inductive I.
+      
+      (* Power set axiom *)
+      Definition encodes_subset (x A : Alphacarrier) : Prop :=
+        is_set_code x /\ is_set_code A /\
+        forall y, mem y x -> mem y A.
+      
+      Definition is_powerset (A ps : Alphacarrier) : Prop :=
+        is_set_code A /\ is_set_code ps /\
+        forall x, mem x ps <-> encodes_subset x A.
+      
+      Axiom powerset_exists : forall A,
+        is_set_code A -> exists ps, is_powerset A ps.
+      
+      (* Replacement axiom *)
+      Definition is_functional (R : Alphacarrier -> Alphacarrier -> Prop) : Prop :=
+        forall x y z, R x y -> R x z -> y = z.
+      
+      Axiom replacement : forall A (R : Alphacarrier -> Alphacarrier -> Prop),
+        is_set_code A ->
+        is_functional R ->
+        exists B, is_set_code B /\
+          forall y, mem y B <-> exists x, mem x A /\ R x y.
+      
+      (* Foundation axiom *)
+      Axiom foundation : forall A,
+        is_set_code A ->
+        (exists x, mem x A) ->
+        exists x, mem x A /\ forall y, mem y x -> ~ mem y A.
+      
+      (* Axiom of choice *)
+      Definition is_family_of_sets (F : Alphacarrier) : Prop :=
+        is_set_code F /\ forall x, mem x F -> is_set_code x.
+      
+      Definition is_choice_function (F f : Alphacarrier) : Prop :=
+        is_family_of_sets F /\ is_set_code f /\
+        forall A, mem A F -> 
+          (exists a, mem a A) ->
+          exists a, mem a A /\ mem (pair_code A a) f.
+      
+      Axiom choice : forall F,
+        is_family_of_sets F ->
+        (forall A, is_set_code A -> In A (set_decode F) -> 
+          exists a, is_set_code a /\ In a (set_decode A)) ->
+        exists f, is_choice_function F f.
+    End ZFCAxioms.
+  End Axioms.
+
+  (** ** Natural Numbers
+      
+      Von Neumann construction of naturals *)
+  Module Naturals.
+    Section NaturalNumbers.
+      Context {H_alpha: ClassicalAlphaType}.
+      Import Basic.
+      Import Fundamental.
+      Import Codes.
+      Import Axioms.
+      
+      Axiom successor_code : Alphacarrier -> Alphacarrier.
+      Axiom successor_code_spec : forall x,
+        is_set_code x -> is_successor x (successor_code x).
+      
+      (* The first few naturals *)
+      Definition zero_zfc := empty_code.
+      Definition one_zfc := successor_code zero_zfc.
+      Definition two_zfc := successor_code one_zfc.
+      Definition three_zfc := successor_code two_zfc.
+      
+      (* Natural numbers are elements of all inductive sets *)
+      Definition is_natural_number (n : Alphacarrier) : Prop :=
+        forall I, is_inductive I -> mem n I.
+      
+      Theorem zero_is_natural : is_natural_number zero_zfc.
+      Proof.
+        unfold is_natural_number, zero_zfc.
+        intros I HI.
+        destruct HI as [HIcode [[e [He [Hemp Hemem]]] Hclosed]].
+        (* Need axiom that empty sets are unique *)
+        Axiom empty_unique : forall e1 e2,
+          is_set_code e1 -> is_set_code e2 ->
+          (forall x, ~ mem x e1) ->
+          (forall x, ~ mem x e2) ->
+          e1 = e2.
+        assert (e = empty_code).
+        { apply empty_unique.
+          - exact He.
+          - destruct empty_code_spec; assumption.
+          - exact Hemp.
+          - exact not_mem_empty. }
+        subst e.
+        exact Hemem.
+      Qed.
+
+    End NaturalNumbers.
+  End Naturals.
+
+  (** ** Russell and Paradoxes
+      
+      How paradoxes are handled in our framework *)
+  Module Paradoxes.
+    Section ParadoxHandling.
+      Context {H_alpha: ClassicalAlphaType}.
+      Import Basic.
+      Import Fundamental.
+      Import Codes.
+      Import Axioms.
+      
+      (* Russell's set *)
+      Definition russell_set : ZSet :=
+        fun x => is_set_code x /\ ~ mem x x.
+      
+      (* Russell's set cannot have a code *)
+      Theorem russell_has_no_code :
+        ~ exists r, is_set_code r /\ set_eq (set_decode r) russell_set.
+      Proof.
+        intros [r [Hr Hdecode]].
+        destruct (alpha_constant_decision (mem r r)) as [Hmem | Hnmem].
+        - assert (In r russell_set).
+          { apply Hdecode. destruct Hmem as [_ H]. exact H. }
+          unfold russell_set, In in H.
+          destruct H as [_ Hnot].
+          exact (Hnot Hmem).
+        - assert (In r russell_set).
+          { unfold russell_set, In. split; assumption. }
+          assert (mem r r).
+          { split; [exact Hr|]. apply Hdecode. exact H. }
+          exact (Hnmem H0).
+      Qed.
+      
+      (* Foundation prevents self-membership *)
+      Theorem no_set_contains_itself : forall x,
+        is_set_code x -> ~ mem x x.
+      Proof.
+        intros x Hx Hmem.
+        destruct (singleton_code_spec x) as [Hs_code Hs_decode].
+        assert (exists y, mem y (singleton_code x)).
+        { exists x. 
+          split.
+          - exact Hs_code.
+          - apply Hs_decode.
+            apply singleton_spec.
+            reflexivity. }
+        destruct (foundation (singleton_code x) Hs_code H) as [y [Hy Hmin]].
+        assert (y = x).
+        { destruct Hy as [_ Hy_in].
+          apply Hs_decode in Hy_in.
+          apply singleton_spec in Hy_in.
+          exact Hy_in. }
+        subst y.
+        apply (Hmin x Hmem).
+        split.
+        - exact Hs_code.
+        - apply Hs_decode. 
+          apply singleton_spec. 
+          reflexivity.
+      Qed.
+    End ParadoxHandling.
+  End Paradoxes.
+
+  (** ** The Hierarchy
+      
+      Building mathematics from the void *)
+  Module Hierarchy.
+    Section CumulativeHierarchy.
+      Context {H_alpha: ClassicalAlphaType}.
+      Import Basic.
+      Import Fundamental.
+      Import Codes.
+      Import Axioms.
+      Import Operations.
+      
+      (* Sets have "rank" - distance from the void *)
+      Definition rank_0_set (x : Alphacarrier) : Prop :=
+        is_set_code x /\ forall y, ~ mem y x.
+      
+      Definition rank_at_most_n : nat -> Alphacarrier -> Prop :=
+        fix rank n x :=
+          match n with
+          | 0 => rank_0_set x
+          | S n' => is_set_code x /\ 
+                    forall y, mem y x -> rank n' y
+          end.
+      
+      Theorem empty_rank_0 : rank_at_most_n 0 empty_code.
+      Proof.
+        unfold rank_at_most_n, rank_0_set.
+        destruct empty_code_spec as [Hcode _].
+        split.
+        - exact Hcode.
+        - exact not_mem_empty.
+      Qed.
+      
+      (* The profound insight: Everything comes from nothing *)
+      Theorem complement_empty_is_universal :
+        set_eq (compl Empty) Universal.
+      Proof.
+        unfold set_eq, ClassicalAlphaProperties.Predicates.pred_equiv.
+        intro x.
+        unfold compl, Empty, Universal, In, 
+              ClassicalAlphaProperties.Helpers.the_necessary.
+        split.
+        - intro H. exact H.
+        - intro H. exact H.
+      Qed.
+    End CumulativeHierarchy.
+  End Hierarchy.
+
+  Module Theorems.
+    Section MainTheorems.
+      Context {H_alpha: ClassicalAlphaType}.
+      Import Basic.
+      Import Fundamental.
+      Import Operations.
+      Import Algebra.
+      Import Codes.
+      Import Axioms.
+      Import Naturals.
+      Import Paradoxes.
+      Import Hierarchy.
+      
+      (** ** Binary Operations via Pairing and Union *)
+      
+      Theorem binary_union_exists : forall A B,
+        is_set_code A -> is_set_code B ->
+        exists U, is_set_code U /\ 
+          forall x, mem x U <-> (mem x A \/ mem x B).
+      Proof.
+        intros A B HA HB.
+        (* First, create the pair {A, B} *)
+        destruct (pair_code_spec A B) as [HP_code HP_decode].
+        (* Then take union of this pair *)
+        destruct (union_exists (pair_code A B) HP_code) as [U HU].
+        exists U.
+        destruct HU as [HF_code [HU_code HU_spec]].
+        split; [exact HU_code|].
+        intro x.
+        split.
+        - intro HxU.
+          apply HU_spec in HxU.
+          destruct HxU as [Y [HYP HxY]].
+          destruct HYP as [_ HYP_in].
+          (* Y is in the pair {A, B} *)
+          assert (In Y (pair A B)).
+          { apply HP_decode. exact HYP_in. }
+          apply pair_spec in H.
+          destruct H as [HYA | HYB].
+          + left. subst Y. exact HxY.
+          + right. subst Y. exact HxY.
+        - intros [HxA | HxB].
+          + apply HU_spec.
+            exists A. split; [|exact HxA].
+            split; [exact HP_code|].
+            apply HP_decode.
+            apply pair_spec. left. reflexivity.
+          + apply HU_spec.
+            exists B. split; [|exact HxB].
+            split; [exact HP_code|].
+            apply HP_decode.
+            apply pair_spec. right. reflexivity.
+      Qed.
+      
+      Theorem intersection_exists : forall A B,
+        is_set_code A -> is_set_code B ->
+        exists I, is_set_code I /\
+          forall x, mem x I <-> (mem x A /\ mem x B).
+      Proof.
+        intros A B HA HB.
+        apply (separation A (fun x => mem x B) HA).
+      Qed.
+      
+      (** ** Function Images via Replacement *)
+      
+      Theorem function_image_exists : forall A f,
+        is_set_code A ->
+        exists B, is_set_code B /\
+          forall y, mem y B <-> exists x, mem x A /\ y = f x.
+      Proof.
+        intros A f HA.
+        (* Define the relation R(x,y) := y = f(x) *)
+        pose (R := fun x y => y = f x).
+        
+        (* Show R is functional *)
+        assert (Hfunc: is_functional R).
+        { unfold is_functional, R.
+          intros x y z Hy Hz.
+          rewrite Hy. symmetry. exact Hz. }
+        
+        (* Apply replacement *)
+        destruct (replacement A R HA Hfunc) as [B [HB HB_spec]].
+        exists B. split; [exact HB|].
+        
+        intros y. split.
+        - intro HyB.
+          apply HB_spec in HyB.
+          destruct HyB as [x [HxA Hy]].
+          exists x. split; [exact HxA|].
+          unfold R in Hy. exact Hy.
+        - intros [x [HxA Heq]].
+          apply HB_spec.
+          exists x. split; [exact HxA|].
+          unfold R. exact Heq.
+      Qed.
+      
+      (** ** Power Set Properties *)
+      
+      Theorem empty_in_every_powerset : forall A ps,
+        is_set_code A -> is_powerset A ps ->
+        mem empty_code ps.
+      Proof.
+        intros A ps HA Hps.
+        destruct Hps as [_ [Hps_code Hps_spec]].
+        apply Hps_spec.
+        unfold encodes_subset.
+        destruct empty_code_spec as [He_code _].
+        split; [exact He_code|].
+        split; [exact HA|].
+        intros y Hy.
+        (* y mem empty_code is impossible *)
+        exfalso.
+        exact (not_mem_empty y Hy).
+      Qed.
+      
+      Theorem set_in_own_powerset : forall A ps,
+        is_set_code A -> is_powerset A ps ->
+        mem A ps.
+      Proof.
+        intros A ps HA Hps.
+        destruct Hps as [_ [Hps_code Hps_spec]].
+        apply Hps_spec.
+        unfold encodes_subset.
+        split; [exact HA|].
+        split; [exact HA|].
+        intros y Hy.
+        (* y mem A -> y mem A is trivial *)
+        exact Hy.
+      Qed.
+      
+      Theorem singleton_in_powerset : forall A ps a,
+        is_set_code A -> is_powerset A ps -> mem a A ->
+        exists sa, is_set_code sa /\ mem sa ps /\
+          forall x, mem x sa <-> x = a.
+      Proof.
+        intros A ps a HA Hps Ha.
+        exists (singleton_code a).
+        destruct (singleton_code_spec a) as [Hsa_code Hsa_decode].
+        split; [exact Hsa_code|].
+        split.
+        - (* singleton a is in powerset *)
+          destruct Hps as [_ [_ Hps_spec]].
+          apply Hps_spec.
+          unfold encodes_subset.
+          split; [exact Hsa_code|].
+          split; [exact HA|].
+          intros x Hx.
+          destruct Hx as [_ Hx_in].
+          assert (In x (singleton a)).
+          { apply Hsa_decode. exact Hx_in. }
+          assert (x = a).
+          { apply singleton_spec. exact H. }
+          rewrite H0.
+          exact Ha.
+        - (* Characterization of singleton *)
+          intros x.
+          split.
+          + intro Hx.
+            destruct Hx as [_ Hx_in].
+            assert (In x (singleton a)).
+            { apply Hsa_decode. exact Hx_in. }
+            apply singleton_spec.
+            exact H.
+          + intro Heq.
+            rewrite Heq.
+            split; [exact Hsa_code|].
+            apply Hsa_decode.
+            apply singleton_spec.
+            reflexivity.
+      Qed.
+      
+      (** ** Natural Number Induction *)
+      
+      (* First we need these axioms *)
+      Axiom nat_set_code : Alphacarrier.
+      Axiom nat_set_code_spec : 
+        is_set_code nat_set_code /\
+        forall n, mem n nat_set_code <-> is_natural_number n.
+      
+      Axiom nat_is_set_code : forall n,
+        is_natural_number n -> is_set_code n.
+      
+      Axiom successor_preserves_nat : forall n,
+        is_natural_number n -> is_natural_number (successor_code n).
+      
+      Theorem nat_induction : forall (P : Alphacarrier -> Prop),
+        P zero_zfc ->
+        (forall n, is_natural_number n -> P n -> P (successor_code n)) ->
+        forall n, is_natural_number n -> P n.
+      Proof.
+        intros P Hz Hsucc n Hn.
+        
+        (* The subset of naturals satisfying P *)
+        destruct nat_set_code_spec as [Hnat_code Hnat_spec].
+        destruct (separation nat_set_code P Hnat_code) as [S [HS HS_spec]].
+        
+        (* Claim: S is inductive *)
+        assert (His_ind: is_inductive S).
+        { unfold is_inductive.
+          split; [exact HS|].
+          split.
+          - (* S contains zero *)
+            exists zero_zfc.
+            split; [|split].
+            + destruct empty_code_spec; assumption.
+            + exact not_mem_empty.
+            + apply HS_spec. split.
+              * apply Hnat_spec. exact zero_is_natural.
+              * exact Hz.
+          - (* S is closed under successor *)
+            intros x HxS.
+            assert (Hx_components: mem x nat_set_code /\ P x).
+            { apply HS_spec. exact HxS. }
+            destruct Hx_components as [Hx_in_nat Px].
+            
+            assert (Hx_nat: is_natural_number x).
+            { apply Hnat_spec. exact Hx_in_nat. }
+            
+            assert (Hx_code: is_set_code x).
+            { apply nat_is_set_code. exact Hx_nat. }
+            
+            exists (successor_code x).
+            split.
+            + apply successor_code_spec. exact Hx_code.
+            + apply HS_spec. split.
+              * apply Hnat_spec. 
+                apply successor_preserves_nat. exact Hx_nat.
+              * apply Hsucc; assumption. }
+        
+        (* Since n is natural, it's in S *)
+        assert (n_in_S: mem n S).
+        { unfold is_natural_number in Hn.
+          exact (Hn S His_ind). }
+        
+        (* Therefore P n holds *)
+        apply HS_spec in n_in_S.
+        destruct n_in_S as [_ Pn].
+        exact Pn.
+      Qed.
+      
+      (** ** Cantor's Theorem - The Crown Jewel *)
+      
+      (* Helper for converting between different membership notions *)
+      Lemma mem_iff_is_member : forall a b,
+        mem a b <-> is_set_code b /\ In a (set_decode b).
+      Proof.
+        intros a b.
+        split; intro H; exact H.
+      Qed.
+      
+      Theorem cantor_theorem : forall A ps,
+        is_set_code A -> is_powerset A ps ->
+        ~ exists f : Alphacarrier -> Alphacarrier,
+          (forall x, mem x A -> mem (f x) ps) /\
+          (forall y, mem y ps -> exists x, mem x A /\ y = f x).
+      Proof.
+        intros A ps HA Hps [f [Hf_maps Hf_onto]].
+        
+        (* Define the diagonal set D = {x ∈ A | x ∉ f(x)} *)
+        destruct (separation A (fun x => ~ mem x (f x)) HA) as [D [HD HD_spec]].
+        
+        (* D is a subset of A, so D ∈ P(A) *)
+        assert (HD_in_ps: mem D ps).
+        { destruct Hps as [_ [_ Hps_spec]].
+          apply Hps_spec.
+          unfold encodes_subset.
+          split; [exact HD|].
+          split; [exact HA|].
+          intros y Hy.
+          apply HD_spec in Hy.
+          destruct Hy as [H_mem_A _].
+          exact H_mem_A. }
+        
+        (* Since f is onto, D = f(d) for some d ∈ A *)
+        destruct (Hf_onto D HD_in_ps) as [d [Hd Heq]].
+        
+        (* Now the contradiction: d ∈ D ↔ d ∉ f(d) = D *)
+        destruct (alpha_constant_decision (mem d D)) as [Hd_in | Hd_out].
+        - (* d ∈ D, so d ∉ f(d) = D, contradiction *)
+          assert (H_contra : mem d A /\ ~ mem d (f d)).
+          { apply HD_spec. exact Hd_in. }
+          destruct H_contra as [_ Hnot_fd].
+          rewrite Heq in Hd_in.
+          exact (Hnot_fd Hd_in).
+        - (* d ∉ D, so by definition of D, d ∈ f(d) = D *)
+          assert (mem d D).
+          { apply HD_spec.
+            split.
+            + exact Hd.
+            + rewrite <- Heq. exact Hd_out. }
+          exact (Hd_out H).
+      Qed.
+      
+      (** ** Rank and Hierarchy Properties *)
+      
+      Theorem singleton_rank_1 : forall a,
+        rank_at_most_n 0 a ->
+        rank_at_most_n 1 (singleton_code a).
+      Proof.
+        intros a H0.
+        simpl.
+        destruct (singleton_code_spec a) as [Hcode Hdecode].
+        split; [exact Hcode|].
+        intros y Hy.
+        (* mem y (singleton_code a) means y = a *)
+        destruct Hy as [_ Hy_in].
+        assert (In y (singleton a)) by (apply Hdecode; exact Hy_in).
+        assert (y = a) by (apply singleton_spec; exact H).
+        subst y.
+        exact H0.
+      Qed.
+    End MainTheorems.
+  End Theorems.
+End ZFC.
 
 
-(* The profound connection: Well-founded sets are those with finite "distance" from void *)
-Definition has_finite_rank (x : Alphacarrier) : Prop :=
-  exists n, rank_at_most_n n x.
+(** * ZFC Metatheory *)
 
-(* All natural numbers (as von Neumann ordinals) have finite rank *)
-Theorem naturals_have_finite_rank : forall n,
-  is_natural_number n -> has_finite_rank n.
-Proof.
-  intros n Hn.
-  apply (nat_induction_zfc (fun n => has_finite_rank n)).
-  - (* Base: zero has rank 0 *)
-    exists 0. apply empty_rank_0.
-  - (* Step: if n has rank k, then S(n) has rank at most k+2 *)
-    intros m Hm [k Hk].
-    exists (S (S k)).
-    (* Proof would show successor adds at most 2 to rank *)
-Admitted.
+Module ZFCMeta.
+  Section Metatheory.
+    Context {H_alpha: ClassicalAlphaType}.
+    Import ZFC.Basic.
+    Import ZFC.Fundamental.
+    Import ZFC.Operations.
+    Import ZFC.Codes.
+    Import ZFC.Axioms.
+    
+    (** ** Uniqueness Results *)
+    
+    (* Key axiom: codes are extensional *)
+    Axiom code_extensionality : forall c1 c2,
+      is_set_code c1 -> is_set_code c2 ->
+      set_eq (set_decode c1) (set_decode c2) ->
+      c1 = c2.
+    
+    (* Empty sets are unique *)
+    Theorem empty_unique : forall e1 e2,
+      is_set_code e1 -> is_set_code e2 ->
+      (forall x, ~ mem x e1) ->
+      (forall x, ~ mem x e2) ->
+      e1 = e2.
+    Proof.
+      intros e1 e2 He1 He2 Hemp1 Hemp2.
+      apply code_extensionality; try assumption.
+      unfold set_eq, ClassicalAlphaProperties.Predicates.pred_equiv.
+      intro x.
+      split; intro Hx; exfalso.
+      - apply (Hemp1 x). split; [exact He1 | exact Hx].
+      - apply (Hemp2 x). split; [exact He2 | exact Hx].
+    Qed.
+    
+    (* Powersets are unique *)
+    Theorem powerset_unique : forall A ps1 ps2,
+      is_powerset A ps1 -> is_powerset A ps2 ->
+      ps1 = ps2.
+    Proof.
+      intros A ps1 ps2 Hps1 Hps2.
+      destruct Hps1 as [HA1 [Hps1_code Hps1_spec]].
+      destruct Hps2 as [HA2 [Hps2_code Hps2_spec]].
+      apply code_extensionality; try assumption.
+      unfold set_eq, ClassicalAlphaProperties.Predicates.pred_equiv.
+      intro x.
+      split; intro Hx.
+      - assert (mem x ps1) by (split; [exact Hps1_code | exact Hx]).
+        apply Hps1_spec in H.
+        apply Hps2_spec in H.
+        destruct H as [_ Hx2].
+        exact Hx2.
+      - assert (mem x ps2) by (split; [exact Hps2_code | exact Hx]).
+        apply Hps2_spec in H.
+        apply Hps1_spec in H.
+        destruct H as [_ Hx1].
+        exact Hx1.
+    Qed.
+    
+    (** ** Choice-free Powerset Selection *)
+    
+    (* Since powersets are unique, we can axiomatize a selection function *)
+    Axiom powerset_selector : Alphacarrier -> Alphacarrier.
+    Axiom powerset_selector_spec : forall A,
+      is_set_code A -> is_powerset A (powerset_selector A).
+    
+    (* Every non-empty set contains a member *)
+    Lemma non_empty_has_member : forall x,
+      is_set_code x ->
+      x <> empty_code ->
+      exists y, mem y x.
+    Proof.
+      intros x Hx Hne.
+      apply ClassicalAlphaProperties.Existence.not_all_not_ex.
+      intro Hall_not.
+      apply Hne.
+      apply code_extensionality; try assumption.
+      - destruct empty_code_spec; assumption.
+      - unfold set_eq, ClassicalAlphaProperties.Predicates.pred_equiv.
+        intro z.
+        split; intro Hz.
+        + (* z ∈ set_decode x → z ∈ set_decode empty_code *)
+          exfalso.
+          apply (Hall_not z).
+          split; [exact Hx | exact Hz].
+        + (* z ∈ set_decode empty_code → z ∈ set_decode x *)
+          destruct empty_code_spec as [_ Hempty_decode].
+          apply Hempty_decode in Hz.
+          unfold In, Empty in Hz.
+          exfalso.
+          exact (ClassicalAlphaProperties.Core.classical_veil_is_impossible z Hz).
+    Qed.
+    
+  End Metatheory.
+End ZFCMeta.
 
-(* The ultimate insight: The cumulative hierarchy V is built in stages from void *)
-(* V_0 = ∅ = classical_veil *)
-(* V_1 = P(V_0) = {∅} *)
-(* V_2 = P(V_1) = {∅, {∅}} *)
-(* ... *)
-(* Each level adds one more "layer" of distance from impossibility *)
+(** * Complete Theorems *)
 
-Theorem cumulative_hierarchy_from_void :
-  exists V : nat -> Alphacarrier,
-    V 0 = empty_code /\
-    forall n, is_powerset (V n) (V (S n)).
-Proof.
-  (* This would construct the entire set-theoretic universe from classical_veil *)
-  (* The construction exists by iterating powerset, starting from void *)
-Admitted.
+Module ZFCComplete.
+  Section CompleteTheorems.
+    Context {H_alpha: ClassicalAlphaType}.
+    Import ZFC.Basic ZFC.Fundamental ZFC.Operations ZFC.Codes ZFC.Axioms.
+    Import ZFC.Naturals ZFC.Hierarchy.
+    Import ZFC.Theorems.
+    Import ZFCMeta.
+    
+    Theorem math_emerges_from_void : 
+      exists (hierarchy : nat -> Alphacarrier),
+        hierarchy 0 = empty_code /\
+        (forall n, is_set_code (hierarchy n)) /\
+        (forall n, is_powerset (hierarchy n) (hierarchy (S n))).
+    Proof.
+      (* Define hierarchy using the selector *)
+      exists (fix hierarchy n :=
+        match n with
+        | 0 => empty_code
+        | S n' => powerset_selector (hierarchy n')
+        end).
+      
+      split; [reflexivity|].
+      split.
+      - (* Each level is a set code *)
+        intro n.
+        induction n.
+        + simpl. destruct empty_code_spec; assumption.
+        + simpl. 
+          destruct (powerset_selector_spec _ IHn) as [_ [Hcode _]].
+          exact Hcode.
+      - (* Each successor is the powerset *)
+        intro n.
+        simpl.
+        apply powerset_selector_spec.
+        induction n.
+        + simpl. destruct empty_code_spec; assumption.
+        + simpl.
+          destruct (powerset_selector_spec _ IHn) as [_ [Hcode _]].
+          exact Hcode.
+    Qed.
+    
+    Lemma nth_beyond_length : forall {A} (l : list A) n (default : A),
+      length l <= n -> nth n l default = default.
+    Proof.
+      intros A l n default Hlen.
+      generalize dependent n.
+      induction l; intros n Hlen.
+      - (* l = [] *)
+        destruct n; reflexivity.
+      - (* l = a :: l' *)
+        destruct n.
+        + simpl in Hlen. lia.
+        + simpl. apply IHl. simpl in Hlen. lia.
+    Qed.
 
-(* Final insight: Every set in ZFC has a "impossibility genealogy" - 
-   a finite path back to the omega veil through membership *)
-(* Theorem everything_comes_from_nothing :
-  forall x, has_finite_rank x ->
-  exists (path : list Alphacarrier),
-    last path empty_code = x /\
-    forall i, i < length path - 1 ->
-      is_member (nth i path empty_code) (nth (i+1) path empty_code).
-Proof.
-  (* This would show every well-founded set has a membership chain to empty *)
-  (* The proof would use induction on rank *)
-Admitted. *)
+    Lemma nth_in_bounds : forall {A} (l : list A) n (default x : A),
+      nth n l default = x ->
+      x <> default ->
+      n < length l.
+    Proof.
+      intros A l n default x Hnth Hneq.
+      destruct (lt_dec n (length l)); [assumption|].
+      exfalso.
+      assert (nth n l default = default).
+      { apply nth_beyond_length. lia. }
+      congruence.
+    Qed.
 
+    (* Specific to our use case *)
+    Lemma chain_element_not_empty : forall chain n z,
+      nth n chain empty_code = z ->
+      n > 0 ->
+      mem z empty_code ->
+      False.
+    Proof.
+      intros chain n z Hnth Hn Hz.
+      exact (not_mem_empty z Hz).
+    Qed.
 
-End ZFC_in_ClassicalAlpha.
+    Lemma chain_length_bound : forall chain n z,
+      nth n chain empty_code = z ->
+      n > 0 ->
+      (exists y, mem z y) ->  
+      length chain > n.
+    Proof.
+      (* This is a technical detail about how we represent chains.
+        In a cleaner formulation, we'd ensure chains have the right length by construction. *)
+      admit.
+    Admitted.
+    
+    (** ** Well-founded Membership *)
+    (* The membership relation is well-founded *)
+    Axiom mem_well_founded : forall P : Alphacarrier -> Prop,
+      (forall x, is_set_code x -> 
+        (forall y, mem y x -> P y) -> P x) ->
+      forall x, is_set_code x -> P x.
+    
+    Theorem void_generates_all : forall x,
+      is_set_code x ->
+      x = empty_code \/
+      exists n, n > 0 /\ 
+        exists chain : list Alphacarrier,
+          nth 0 chain empty_code = empty_code /\
+          nth n chain empty_code = x /\
+          forall i, i < n ->
+            mem (nth i chain empty_code) (nth (S i) chain empty_code).
+    Proof.
+      intros x Hx.
+      (* Use well-founded induction on membership *)
+      revert Hx.
+      apply (mem_well_founded (fun x => x = empty_code \/
+        exists n, n > 0 /\ 
+          exists chain : list Alphacarrier,
+            nth 0 chain empty_code = empty_code /\
+            nth n chain empty_code = x /\
+            forall i, i < n ->
+              mem (nth i chain empty_code) (nth (S i) chain empty_code))).
+      
+      intros y Hy IH.
+      destruct (alpha_constant_decision (y = empty_code)) as [Heq | Hne].
+      - (* y is empty *)
+        left. exact Heq.
+      - (* y is non-empty *)
+        right.
+        destruct (non_empty_has_member y Hy Hne) as [z [Hz_code Hz_mem]].
+        destruct (IH z (conj Hz_code Hz_mem)) as [Hz_empty | [n [Hn [chain Hchain]]]].
+        + (* z is empty: chain is [empty_code; y] *)
+          exists 1.
+          split; [lia|].
+          exists [empty_code; y].
+          split; [reflexivity|].
+          split; [reflexivity|].
+          intros i Hi.
+          assert (i = 0) by lia.
+          subst i. simpl.
+          rewrite <- Hz_empty.
+          split; assumption.
+        + (* z has a chain: extend it with y *)
+          destruct Hchain as [Hstart [Hend Hlinks]].
+          (* Get the length bound we need *)
+          assert (Hlen: length chain > n).
+          { apply chain_length_bound with z.
+            - exact Hend.
+            - exact Hn.
+            - exists y. split; assumption. }
+
+          exists (S n).
+          split; [lia|].
+          exists (chain ++ [y]).
+          split.
+          * (* Start is still empty_code *)
+            rewrite app_nth1.
+            -- exact Hstart.
+            -- lia.
+          * split.
+            -- (* End is y: need to show nth (S n) (chain ++ [y]) empty_code = y *)
+              (* This requires reasoning about the relationship between n and length chain *)
+              admit.
+            -- (* Links: need to show forall i < S n, mem (nth i ...) (nth (S i) ...) *)
+              (* This requires splitting into cases for old links and the new z->y link *)
+              admit.
+    Admitted.
+
+    (** The philosophical culmination *)
+    Theorem mathematics_from_void : 
+      (exists hierarchy : nat -> Alphacarrier,
+        hierarchy 0 = empty_code /\
+        (forall n, is_set_code (hierarchy n)) /\
+        (forall n, is_powerset (hierarchy n) (hierarchy (S n)))) /\
+      (forall x, is_set_code x -> 
+        x = empty_code \/ 
+        exists n chain, 
+          nth 0 chain empty_code = empty_code /\
+          nth n chain empty_code = x /\
+          n > 0 /\
+          forall i, i < n -> mem (nth i chain empty_code) (nth (S i) chain empty_code)).
+    Proof.
+      split.
+      - exact math_emerges_from_void.
+      - intros x Hx.
+        destruct (void_generates_all x Hx) as [Heq | [n [Hn [chain Hchain]]]].
+        + left. exact Heq.
+        + right. 
+          exists n, chain.
+          destruct Hchain as [H0 [Hend Hlinks]].
+          split; [exact H0|].
+          split; [exact Hend|].
+          split; [exact Hn|].
+          exact Hlinks.
+    Qed.
+  End CompleteTheorems.
+End ZFCComplete.
